src/n-bit/wordsLib.sig
@@ -2,33 +2,96 @@ signature wordsLib =
 sig
     include Abbrev
 
-    val words_compset : unit -> computeLib.compset
+    val words_compset     : unit -> computeLib.compset
 
-    val SIZES_ss      : simpLib.ssfrag
+    val SIZES_ss          : simpLib.ssfrag
+    val BIT_ss            : simpLib.ssfrag
 
-    val mk_word_size  : int -> unit
+    val WORD_GROUND_ss    : simpLib.ssfrag
+    val WORD_ARITH_ss     : simpLib.ssfrag
+    val WORD_LOGIC_ss     : simpLib.ssfrag
+    val WORD_SHIFT_ss     : simpLib.ssfrag
+    val WORD_ARITH_EQ_ss  : simpLib.ssfrag
+    val WORD_BIT_EQ_ss    : simpLib.ssfrag
+    val WORD_EXTRACT_ss   : simpLib.ssfrag
+    val WORD_MUL_LSL_ss   : simpLib.ssfrag
 
-    val SIZES_CONV    : conv
-    val WORDS_CONV    : conv
-    val WORDS_RULE    : rule
-    val WORDS_TAC     : tactic
+    val WORD_ss           : simpLib.ssfrag
 
-    val WORDS_EMIT_RULE : rule
+    val SIZES_CONV        : conv
 
-    val Cases_on_word : term frag list -> tactic
-    val Cases_word    : tactic
+    val WORD_ARITH_CONV   : conv
+    val WORD_LOGIC_CONV   : conv
+    val WORD_MUL_LSL_CONV : conv
+    val WORD_CONV         : conv
+    val WORD_BIT_EQ_CONV  : conv
+    val WORD_EVAL_CONV    : conv
 
-    val pp_word       : (hol_type -> StringCvt.radix) -> unit
+    val WORD_DP           : conv -> conv
+    val WORD_DECIDE       : conv
 
-    val pp_word_bin   : unit -> unit
-    val pp_word_oct   : unit -> unit
-    val pp_word_hex   : unit -> unit
-    val pp_word_dec   : unit -> term_pp_types.userprinter option
+    val mk_word_size      : int -> unit
+
+    val WORD_EVAL_RULE    : rule
+    val WORD_EVAL_TAC     : tactic
+
+    val WORDS_EMIT_RULE   : rule
+
+    val Cases_on_word     : term frag list -> tactic
+    val Cases_word        : tactic
+
+    val pp_word           : (hol_type -> StringCvt.radix) -> unit
+
+    val pp_word_bin       : unit -> unit
+    val pp_word_oct       : unit -> unit
+    val pp_word_hex       : unit -> unit
+    val pp_word_dec       : unit -> term_pp_types.userprinter option
+
+    val prefer_word       : unit -> unit
+    val deprecate_word    : unit -> unit
 
     val notify_word_length_guesses : bool ref
     val guess_word_lengths         : term -> term
     val guess_lengths              : unit -> unit
 
-    val prefer_word    : unit -> unit
-    val deprecate_word : unit -> unit
+(*
+    [SIZES_ss] evaluates dimindex(:N), dimword(:N) etc.
+
+    [BIT_ss] converts BIT n N to set membership e.g.
+             ``BIT n 3`` to ``n IN {0; 1}``
+
+    [WORD_GROUND_ss] does some ground evaluation
+
+    [WORD_ARITH_ss] AC simplification for *, +, - etc.
+
+    [WORD_LOGIC_ss] AC simplification for &&, !!, ~ etc.
+
+    [WORD_SHIFT_ss] is a basic simpset for word shifts
+
+    [WORD_ss] contains all of the above simpsets
+
+    [WORD_ARITH_EQ_ss] simplifies (a = b) to (a - b = 0w)
+
+    [WORD_BIT_EQ_ss] converts word equality to bitwise equality e.g.
+       ``a !! b << 2 = c:word3`` goes to
+       ``(a %% 2 \/ b %% 0 = c %% 2) /\ (a %% 1 = c %% 1) /\
+         (a %% 0 = c %% 0)``
+
+    [WORD_EXTRACT_ss] is a fairly aggressive simpset for bit extractions
+       ><, <>, --, w2w, sw2w, >>>, >>, #>>, @@ etc.
+
+    [WORD_MUL_LSL_ss] converts products to left shifts e.g. ``4w * a`` goes
+       to ``a << 2`` and ``5w * a`` to ``a << 2 + a``.
+
+    [WORD_ARITH_CONV] is bases on WORD_ARITH_ss and WORD_ARITH_EQ_ss
+
+    [WORD_LOGIC_CONV] is bases on WORD_LOGIC_ss
+
+    [WORD_CONV] is based on WORD_ss
+
+    [WORD_DECIDE] is a decision procedure based on DECIDE
+
+    [WORDS_EMIT_RULE] apply to word theorems when exporting with EmitML
+*)
+
 end
