examples/dev/sw2/regAlloc.sml
@@ -653,6 +653,10 @@ fun args_env args =
 (* alpha-equivalent to the source program.                                   *)
 (*---------------------------------------------------------------------------*)
 
+fun preset_regs tm = 
+ let fun find tm acc =
+      if is_let tm
+
 fun reg_alloc def =
  let
    val (fname, fbody) = dest_eq (concl def)
