src/list/src/selftest.sml
@@ -1,0 +1,29 @@
+open HolKernel Parse boolLib
+open ListConv1
+
+fun test nm cmp pr f (x, expected) = let
+  val _ = print (StringCvt.padRight #" " 20 nm)
+  val _ = print (StringCvt.padRight #" " 40 (pr x))
+  val result = f x
+in
+  if cmp(rhs (concl result),expected) = EQUAL andalso null (hyp result) then
+    (print "OK\n"; true)
+  else (print "FAILED\n"; false)
+end
+
+val _ =
+    if List.all (test "FIRSTN_CONV" Term.compare term_to_string FIRSTN_CONV)
+                [(``FIRSTN 3 [1;2;3;4;5]``, ``[1;2;3]``),
+                 (``FIRSTN 4 [1;2;3;4]``, ``[1;2;3;4]``),
+                 (``FIRSTN 0 [1;2]``, ``[] : num list``),
+                 (``FIRSTN 0 [] : num list``, ``[] : num list``)]
+       andalso
+       List.all
+           (test "BUTFIRSTN_CONV" Term.compare term_to_string BUTFIRSTN_CONV)
+           [(``BUTFIRSTN 3 [1;2;3;4]``, ``[4]``),
+            (``BUTFIRSTN 0 [1;2]``, ``[1;2]``),
+            (``BUTFIRSTN 3 [1;2;3]``, ``[] : num list``),
+            (``BUTFIRSTN 0 [] : num list``, ``[] : num list``)]
+    then
+      Process.exit Process.success
+    else Process.exit Process.failure
